src/coupon_collector/SimpleCouponCollector.lean
@@ -1,129 +1,124 @@
 -- This module serves as the root of the `CouponCollector` library.
--- Import modules here that should be built as part of the library.
-import Paperproof --tool to visualize proofs (I recommend to our group)
-
-/-
-Revised implementatin following Monday's meeting
--/
-
-
-structure Tag where 
-  lhs : UInt8 
-  rhs : UInt8 
-deriving Repr 
-
-
--- Explicit operations user can request (same names as constructors)
-inductive Request --exposed to user
-| Identity : UInt8 → Request
-| Symmetry : Tag → Request
-| Transitivity: Tag → Tag → Request --a structure: multi-args
-
-def apply_coupon_collector : Request → Option Tag
-| Request.Identity x       => some ({lhs := x, rhs := x})
-| Request.Symmetry t       => some ({lhs := t.rhs, rhs := t.lhs})
-| Request.Transitivity t₁ t₂ => if t₁.rhs == t₂.lhs then some {lhs := t₁.lhs, rhs := t₂.rhs} else none
-
-
-
-/-------------------------------------------------------------------- 
-valid/true inputs (tags) and outputs (tags) below
-
-pre: all tag inputs are true; 
-post: all tag outputs are true; 
-
-true tag: lhs == rhs 
--- pre-condition: list [0, 1, 2 tags], just the tag input t: lhs == rhs 
--- post: [0 1 tags] after we apply the function 
--- post: we want to add a separate lean equal condition for post condition, because we 
--- want to use it to assert post condition holds
-----------------------------------------------------------------------/
-
-/- -----------------------------------------------------------------------
-Lean distiguishes == v.s. =
-functionA==functionB cannot be true, even if the output is the same; 
-But functionA=functionB can be true in Lean if the output is equal; 
-we use ==, because we want our proposition to guarantee boolean equality on both value and type. 
-x==y is the same as BEq.beq x y
---------------------------------------------------------------------------/
-
-
-
-/- -----------------------------------------------------------------------------
-Two ways to implement tag_invariant: check every tag in the Tag list that lhs==rhs
-
-def tag_check (ts : List Tag) : Bool :=
-  ts.countP (fun t => t.lhs == t.rhs) == ts.length
-
-From meeting: pre post should be the same 
----------------------------------------------------------------------------------/
-
-
--- https://lean-lang.org/functional_programming_in_lean/getting-to-know/conveniences.html
-def all_tag_true(ts : List Tag) : Bool := -- inputs/ouputs are always true (lhs == rhs
-  ts.all λ t => t.lhs = t.rhs 
+ -- Import modules here that should be built as part of the library.
+ -- import Paperproof --tool to visualize proofs (I recommend to our group)
  
--- define a member function for request
+ /-
+ Revised implementatin following Monday's meeting
+ -/
+ 
+ 
+ structure Tag where 
+   lhs : UInt8 
+   rhs : UInt8 
+ deriving Repr 
+ 
+ 
+ -- Explicit operations user can request (same names as constructors)
+ inductive Request --exposed to user
+ | Identity : UInt8 → Request
+ | Symmetry : Tag → Request
+ | Transitivity: Tag → Tag → Request --a structure: multi-args
+ 
+ def apply_coupon_collector : Request → Option Tag
+ | Request.Identity x       => some ({lhs := x, rhs := x})
+ | Request.Symmetry t       => some ({lhs := t.rhs, rhs := t.lhs})
+ | Request.Transitivity t₁ t₂ => if t₁.rhs == t₂.lhs then some {lhs := t₁.lhs, rhs := t₂.rhs} else none
+ 
+ 
+ -- https://lean-lang.org/functional_programming_in_lean/getting-to-know/conveniences.html
+ def all_tag_true (ts : List Tag) : Bool := -- inputs/ouputs are always true (lhs == rhs
+   ts.all λ t => t.lhs = t.rhs 
+ 
+ -- define a member function for request
+ 
+ def request_to_list : Request -> List Tag --helper function 
+   | Request.Identity _      => [] 
+   | Request.Symmetry t       => [t] 
+   | Request.Transitivity t₁ t₂ => [t₁, t₂]
+ 
+ theorem soundness_proof :
+     ∀ (r : Request), --for all user requests
+     all_tag_true (request_to_list r) → -- if the tag inputs to requests are true, it implies that 
+     all_tag_true ((apply_coupon_collector r).toList) := --the tag outputs from apply_coupon_collector are true
+ by
+   intros r h
+   cases r with
+   | Identity x =>   
+     simp [request_to_list, all_tag_true,  apply_coupon_collector]
+ 
+ 
+   | Symmetry t =>
+     simp [apply_coupon_collector, request_to_list, all_tag_true] at h
+     -- tag_check [t] = (t.lhs = t.rhs), so we can use h directly
+     simp [apply_coupon_collector, all_tag_true]
+     -- now the result is [ { lhs := t.rhs, rhs := t.lhs } ]
+     -- and we want to prove t.rhs = t.lhs, which is just the symmetry of h
+     exact Eq.symm h
+ 
+   | Transitivity t₁ t₂ =>
+   -- simplify h by decomposing  a request list via all_tag_true: unfold a list of true tag
+   simp [request_to_list, all_tag_true] at h
+   by_cases cond : t₁.rhs == t₂.lhs
+   case pos =>
+     let expected : Tag := { lhs := t₁.lhs, rhs := t₂.rhs } -- proof goal 
+     have h_eq : t₁.rhs = t₂.lhs := of_decide_eq_true cond  -- transitivity condition 
+     have lhs_eq_rhs : expected.lhs = expected.rhs := by 
+       calc
+         t₁.lhs = t₁.rhs := h.left
+         _      = t₂.lhs := h_eq
+         _      = t₂.rhs := h.right
+ 
+     simp [apply_coupon_collector, Option.toList, cond, all_tag_true]
+     rw [lhs_eq_rhs]
+ 
+   case neg =>
+     simp [apply_coupon_collector, cond, Option.toList]
+     rfl
+ 
+ 
+ 
+ 
+ 
+ 
+ /- ----------------
+ Some tests below: 
+ ------------------/
+ -- We can write arbitrary code in lean, but it will not satisfy the pre-conditions 
+  --def evilTag (x : UInt8) : Tag := { lhs := x, rhs := 50 }
+ 
+ -- now the evilTag will not create a tag satisfying either of our pre-conditions
+ 
+ --pre_condition r (evilTag x) x
 
-def request_to_list : Request -> List Tag --helper function 
-  | Request.Identity _      => [] 
-  | Request.Symmetry t       => [t] 
-  | Request.Transitivity t₁ t₂ => [t₁, t₂]
-
-
-theorem soundness_proof :
-    ∀ (r : Request), --for all user requests
-    all_tag_true (request_to_list r) → -- if the tag inputs to requests are true, it implies that 
-    all_tag_true ((apply_coupon_collector r).toList) := --the tag outputs from apply_coupon_collector are true
-by
-  intros r h
-  cases r with
-  | Identity x =>   
-    simp [request_to_list, all_tag_true,  apply_coupon_collector]
-
-
-  | Symmetry t =>
-    simp [request_to_list, all_tag_true] at h
-    -- tag_check [t] = (t.lhs = t.rhs), so we can use h directly
-    simp [apply_coupon_collector, all_tag_true]
-    -- now the result is [ { lhs := t.rhs, rhs := t.lhs } ]
-    -- and we want to prove t.rhs = t.lhs, which is just the symmetry of h
-    exact Eq.symm h
-
-  | Transitivity t₁ t₂ =>
-  -- simplify h by decomposing  a request list via all_tag_true: unfold a list of true tag
-  simp [request_to_list, all_tag_true] at h
-  by_cases cond : t₁.rhs == t₂.lhs
-  case pos =>
-    let expected : Tag := { lhs := t₁.lhs, rhs := t₂.rhs } -- proof goal 
-    have h_eq : t₁.rhs = t₂.lhs := of_decide_eq_true cond  -- transitivity condition 
-    have lhs_eq_rhs : expected.lhs = expected.rhs := by 
-      calc
-        t₁.lhs = t₁.rhs := h.left
-        _      = t₂.lhs := h_eq
-        _      = t₂.rhs := h.right
-
-    simp [apply_coupon_collector, Option.toList, cond, all_tag_true]
-    rw [lhs_eq_rhs]
-
-  case neg =>
-    simp [apply_coupon_collector, cond, Option.toList]
-    rfl
-
-    
-
-      
-    
-    
-/- ----------------
-Some tests below: 
-------------------/
--- We can write arbitrary code in lean, but it will not satisfy the pre-conditions 
- --def evilTag (x : UInt8) : Tag := { lhs := x, rhs := 50 }
-
--- now the evilTag will not create a tag satisfying either of our pre-conditions
-
---pre_condition r (evilTag x) x
-
-
--- completeness by proving the converse: if not valid tags/requests -> apply returns no
+-- some study notes below: 
+ /-------------------------------------------------------------------- 
+ valid/true inputs (tags) and outputs (tags) below
+ 
+ pre: all tag inputs are true; 
+ post: all tag outputs are true; 
+ 
+ true tag: lhs == rhs 
+ -- pre-condition: list [0, 1, 2 tags], just the tag input t: lhs == rhs 
+ -- post: [0 1 tags] after we apply the function 
+ -- post: we want to add a separate lean equal condition for post condition, because we 
+ -- want to use it to assert post condition holds
+ ----------------------------------------------------------------------/
+ 
+ /- -----------------------------------------------------------------------
+ Lean distiguishes == v.s. =
+ functionA==functionB cannot be true, even if the output is the same; 
+ But functionA=functionB can be true in Lean if the output is equal; 
+ we use ==, because we want our proposition to guarantee boolean equality on both value and type. 
+ x==y is the same as BEq.beq x y
+ --------------------------------------------------------------------------/
+ 
+ 
+ 
+ /- -----------------------------------------------------------------------------
+ Two ways to implement tag_invariant: check every tag in the Tag list that lhs==rhs
+ 
+ def tag_check (ts : List Tag) : Bool :=
+   ts.countP (fun t => t.lhs == t.rhs) == ts.length
+ 
+ From meeting: pre post should be the same 
+ ---------------------------------------------------------------------------------/
